term

Arithmetization/ISigmaOne/Metamath/Term/Functions.lean
@@ -101,7 +101,7 @@ lemma termSubstVec_cons {k t ts : V} (ht : L.IsUTerm t) (hts : L.IsUTermVec k ts
     L.termSubstVec 2 w ?[t₁, t₂] = ?[L.termSubst w t₁, L.termSubst w t₂] := by
   rw [show (2 : V) = 0 + 1 + 1  by simp [one_add_one_eq_two], termSubstVec_cons] <;> simp [*]
 
-@[simp] lemma termSubst_rng_semiterm {t} (hw : L.IsSemitermVec n m w) (ht : L.IsSemiterm n t) : L.IsSemiterm m (L.termSubst w t) := by
+@[simp] lemma Language.IsSemitermVec.termSubst {t} (hw : L.IsSemitermVec n m w) (ht : L.IsSemiterm n t) : L.IsSemiterm m (L.termSubst w t) := by
   apply Language.IsSemiterm.induction 𝚺 ?_ ?_ ?_ ?_ t ht
   · definability
   · intro z hz; simpa using hw.nth hz
@@ -111,9 +111,12 @@ lemma termSubstVec_cons {k t ts : V} (ht : L.IsUTerm t) (hts : L.IsUTermVec k ts
     exact Language.IsSemitermVec.iff.mpr
       ⟨by simp [hv.isUTerm], fun i hi ↦ by rw [nth_termSubstVec hv.isUTerm hi]; exact ih i hi⟩
 
+@[simp] lemma Language.IsUTermVec.termSubst {t} (hw : L.IsUTermVec n w) (ht : L.IsSemiterm n t) : L.IsUTerm (L.termSubst w t) :=
+  Language.IsSemitermVec.termSubst hw.isSemitermVec ht |>.isUTerm
+
 @[simp] lemma Language.IsSemitermVec.termSubstVec {k n m v} (hw : L.IsSemitermVec n m w) (hv : L.IsSemitermVec k n v) :
     L.IsSemitermVec k m (L.termSubstVec k w v) := Language.IsSemitermVec.iff.mpr
-  ⟨by simp [hv.isUTerm], fun i hi ↦ by rw [nth_termSubstVec hv.isUTerm hi]; exact termSubst_rng_semiterm hw (hv.nth hi)⟩
+  ⟨by simp [hv.isUTerm], fun i hi ↦ by rw [nth_termSubstVec hv.isUTerm hi]; exact hw.termSubst (hv.nth hi)⟩
 
 @[simp] lemma substs_nil {t} (ht : L.IsSemiterm 0 t) : L.termSubst 0 t = t := by
   apply Language.IsSemiterm.induction 𝚺 ?_ ?_ ?_ ?_ t ht
@@ -241,42 +244,43 @@ lemma termShiftVec_cons {k t ts : V} (ht : L.IsUTerm t) (hts : L.IsUTermVec k ts
     L.termShiftVec 1 ?[t₁] = ?[L.termShift t₁] := by
   rw [show (1 : V) = 0 + 1  by simp, termShiftVec_cons] <;> simp [*]
 
-/--/
-@[simp] lemma termShiftVec_cons₂ {n t₁ t₂ : V} (ht₁ : L.IsSemiterm n t₁) (ht₂ : L.IsSemiterm n t₂) :
-    L.termShiftVec 2 n ?[t₁, t₂] = ?[L.termShift n t₁, L.termShift n t₂] := by
-  rw [show (2 : V) = 0 + 1 + 1  by simp [one_add_one_eq_two], termShiftVec_cons] <;> simp [*]
+@[simp] lemma termShiftVec_cons₂ {t₁ t₂ : V} (ht₁ : L.IsUTerm t₁) (ht₂ : L.IsUTerm t₂) :
+    L.termShiftVec 2 ?[t₁, t₂] = ?[L.termShift t₁, L.termShift t₂] := by
+  rw [show (2 : V) = 0 + 1 + 1  by simp [one_add_one_eq_two], termShiftVec_cons] <;> simp [ht₁, ht₂]
 
-@[simp] lemma Language.IsSemiterm.termShift {t} (ht : L.IsSemiterm n t) : L.IsSemiterm n (L.termShift n t) := by
+@[simp] lemma Language.IsSemiterm.termShift {t} (ht : L.IsSemiterm n t) : L.IsSemiterm n (L.termShift t) := by
   apply Language.IsSemiterm.induction 𝚺 ?_ ?_ ?_ ?_ t ht
   · definability
   · intro z hz; simp [hz]
   · intro x; simp
   · intro k f v hkf hv ih;
-    simp only [hkf, hv, termShift_func, Language.IsSemiterm.func_iff, true_and]
-    exact ⟨by simp [Language.termShiftVec, hv], fun i hi ↦ by
-      rw [nth_termShiftVec hv hi]
-      exact ih i hi⟩
+    simp only [hkf, hv.isUTerm, termShift_func, func, true_and]
+    refine Language.IsSemitermVec.iff.mpr ⟨?_, ?_⟩
+    · simp [termShiftVec, hv.isUTerm]
+    · intro i hi
+      rw [nth_termShiftVec hv.isUTerm hi]
+      exact ih i hi
 
-@[simp] lemma Language.IsSemitermVec.termShiftVec {k n v} (hv : L.IsSemitermVec k n v) : L.IsSemitermVec k n (L.termShiftVec k n v) :=
-  ⟨by simp [Language.termShiftVec, hv], fun i hi ↦ by
-    rw [nth_termShiftVec hv hi]
-    exact (hv.prop hi).termShift⟩
+@[simp] lemma Language.IsSemitermVec.termShiftVec {k n v} (hv : L.IsSemitermVec k n v) : L.IsSemitermVec k n (L.termShiftVec k v) :=
+  Language.IsSemitermVec.iff.mpr
+    ⟨by simp [termShiftVec, hv.isUTerm], fun i hi ↦ by
+      rw [nth_termShiftVec hv.isUTerm hi]; exact (hv.nth hi).termShift⟩
 
 end termShift
 
 namespace TermBShift
 
 def blueprint (pL : LDef) : Language.TermRec.Blueprint pL 0 where
-  bvar := .mkSigma “y n z m w | !qqBvarDef y (z + 1)” (by simp)
-  fvar := .mkSigma “y n x m w | !qqFvarDef y x” (by simp)
-  func := .mkSigma “y n k f v v' m w | !qqFuncDef y k f v'” (by simp)
+  bvar := .mkSigma “y z | !qqBvarDef y (z + 1)” (by simp)
+  fvar := .mkSigma “y x | !qqFvarDef y x” (by simp)
+  func := .mkSigma “y k f v v' | !qqFuncDef y k f v'” (by simp)
 
 variable (L)
 
 def construction : Language.TermRec.Construction V L (blueprint pL) where
-  bvar (_ _ z)        := ^#(z + 1)
-  fvar (_ _ x)        := ^&x
-  func (_ _ k f _ v') := ^func k f v'
+  bvar (_ z)        := ^#(z + 1)
+  fvar (_ x)        := ^&x
+  func (_ k f _ v') := ^func k f v'
   bvar_defined := by intro v; simp [blueprint]
   fvar_defined := by intro v; simp [blueprint]
   func_defined := by intro v; simp [blueprint]; rfl
@@ -289,213 +293,230 @@ open TermBShift
 
 variable (L)
 
-def Language.termBShift (n t : V) : V := (construction L).result ![] n t
+def Language.termBShift (t : V) : V := (construction L).result ![] t
 
-def Language.termBShiftVec (k n v : V) : V := (construction L).resultVec ![] k n v
+def Language.termBShiftVec (k v : V) : V := (construction L).resultVec ![] k v
 
 variable {L}
 
-variable {n : V}
+@[simp] lemma Language.termBShift_bvar (z) :
+    L.termBShift ^#z = ^#(z + 1) := by simp [Language.termBShift, construction]
 
-@[simp] lemma termBShift_bvar {z} (hz : z < n) :
-    L.termBShift n ^#z = ^#(z + 1) := by simp [Language.termBShift, hz, construction]
+@[simp] lemma Language.termBShift_fvar (x) :
+    L.termBShift ^&x = ^&x := by simp [Language.termBShift, construction]
 
-@[simp] lemma termBShift_fvar (x) :
-    L.termBShift n ^&x = ^&x := by simp [Language.termBShift, construction]
-
-@[simp] lemma termBShift_func {k f v} (hkf : L.Func k f) (hv : L.IsSemitermVec k n v) :
-    L.termBShift n (^func k f v) = ^func k f (L.termBShiftVec k n v) := by
+@[simp] lemma Language.termBShift_func {k f v} (hkf : L.Func k f) (hv : L.IsUTermVec k v) :
+    L.termBShift (^func k f v) = ^func k f (L.termBShiftVec k v) := by
   simp [Language.termBShift, construction, hkf, hv]; rfl
 
 section
 
-def _root_.LO.FirstOrder.Arith.LDef.termBShiftDef (pL : LDef) : 𝚺₁.Semisentence 3 :=
-  (blueprint pL).result
+def _root_.LO.FirstOrder.Arith.LDef.termBShiftDef (pL : LDef) : 𝚺₁.Semisentence 2 := (blueprint pL).result
 
-def _root_.LO.FirstOrder.Arith.LDef.termBShiftVecDef (pL : LDef) : 𝚺₁.Semisentence 4 := (blueprint pL).resultVec
+def _root_.LO.FirstOrder.Arith.LDef.termBShiftVecDef (pL : LDef) : 𝚺₁.Semisentence 3 := (blueprint pL).resultVec
 
 variable (L)
 
-lemma termBShift_defined : 𝚺₁-Function₂ L.termBShift via pL.termBShiftDef := by
+lemma Language.termBShift_defined : 𝚺₁-Function₁ L.termBShift via pL.termBShiftDef := by
   intro v; simpa using (construction L).result_defined v
 
-@[simp] lemma eval_termBShiftDef (v : Fin 3 → V) :
-    Semiformula.Evalbm (L := ℒₒᵣ) V v pL.termBShiftDef ↔ v 0 = L.termBShift (v 1) (v 2) := (termBShift_defined L).df.iff v
+instance Language.termBShift_definable : 𝚺₁-Function₁ L.termBShift := L.termBShift_defined.to_definable
 
-instance termBShift_definable : 𝚺₁-Function₂ L.termBShift :=
-  (termBShift_defined L).to_definable
+instance Language.termBShift_definable' : Γ-[i + 1]-Function₁ L.termBShift := L.termBShift_definable.of_sigmaOne
 
-@[definability, simp] instance termBShift_definable' (Γ i) : Γ-[i + 1]-Function₂ L.termBShift := .of_sigmaOne (termBShift_definable L) _ _
-
-lemma termBShiftVec_defined : 𝚺₁-Function₃ L.termBShiftVec via pL.termBShiftVecDef := by
+lemma Language.termBShiftVec_defined : 𝚺₁-Function₂ L.termBShiftVec via pL.termBShiftVecDef := by
   intro v; simpa using (construction L).resultVec_defined v
 
-@[simp] lemma eval_termBShiftVecDef (v : Fin 4 → V) :
-    Semiformula.Evalbm (L := ℒₒᵣ) V v pL.termBShiftVecDef ↔ v 0 = L.termBShiftVec (v 1) (v 2) (v 3) := (termBShiftVec_defined L).df.iff v
+instance Language.termBShiftVec_definable : 𝚺₁-Function₂ L.termBShiftVec := L.termBShiftVec_defined.to_definable
 
-instance termBShiftVec_definable : 𝚺₁-Function₃ L.termBShiftVec :=
-  (termBShiftVec_defined L).to_definable
-
-@[simp, definability] instance termBShiftVec_definable' (Γ i) : Γ-[i + 1]-Function₃ L.termBShiftVec :=
-  .of_sigmaOne (termBShiftVec_definable L) _ _
+instance Language.termBShiftVec_definable' : Γ-[i + 1]-Function₂ L.termBShiftVec := L.termBShiftVec_definable.of_sigmaOne
 
 end
 
-@[simp] lemma len_termBShiftVec {k n ts : V} (hts : L.IsSemitermVec k n ts) :
-    len (L.termBShiftVec k n ts) = k := (construction L).resultVec_lh _ hts
+@[simp] lemma len_termBShiftVec {k ts : V} (hts : L.IsUTermVec k ts) :
+    len (L.termBShiftVec k ts) = k := (construction L).resultVec_lh _ hts
 
-@[simp] lemma nth_termBShiftVec {k n ts i : V} (hts : L.IsSemitermVec k n ts) (hi : i < k) :
-    (L.termBShiftVec k n ts).[i] = L.termBShift n ts.[i] :=
+@[simp] lemma nth_termBShiftVec {k ts i : V} (hts : L.IsUTermVec k ts) (hi : i < k) :
+    (L.termBShiftVec k ts).[i] = L.termBShift ts.[i] :=
   (construction L).nth_resultVec _ hts hi
 
-@[simp] lemma termBShiftVec_nil (n : V) : L.termBShiftVec 0 n 0 = 0 :=
-  (construction L).resultVec_nil ![] _
+@[simp] lemma termBShiftVec_nil : L.termBShiftVec 0 0 = 0 :=
+  (construction L).resultVec_nil ![]
 
-lemma termBShiftVec_cons {k n t ts : V} (ht : L.IsSemiterm n t) (hts : L.IsSemitermVec k n ts) :
-    L.termBShiftVec (k + 1) n (t ∷ ts) = L.termBShift n t ∷ L.termBShiftVec k n ts :=
+lemma termBShiftVec_cons {k t ts : V} (ht : L.IsUTerm t) (hts : L.IsUTermVec k ts) :
+    L.termBShiftVec (k + 1) (t ∷ ts) = L.termBShift t ∷ L.termBShiftVec k ts :=
   (construction L).resultVec_cons ![] hts ht
 
-@[simp] lemma termBShiftVec_cons₁ {n t₁ : V} (ht₁ : L.IsSemiterm n t₁) :
-    L.termBShiftVec 1 n ?[t₁] = ?[L.termBShift n t₁] := by
+@[simp] lemma termBShiftVec_cons₁ {t₁ : V} (ht₁ : L.IsUTerm t₁) :
+    L.termBShiftVec 1 ?[t₁] = ?[L.termBShift t₁] := by
   rw [show (1 : V) = 0 + 1  by simp, termBShiftVec_cons] <;> simp [*]
 
-@[simp] lemma termBShiftVec_cons₂ {n t₁ t₂ : V} (ht₁ : L.IsSemiterm n t₁) (ht₂ : L.IsSemiterm n t₂) :
-    L.termBShiftVec 2 n ?[t₁, t₂] = ?[L.termBShift n t₁, L.termBShift n t₂] := by
+@[simp] lemma termBShiftVec_cons₂ {t₁ t₂ : V} (ht₁ : L.IsUTerm t₁) (ht₂ : L.IsUTerm t₂) :
+    L.termBShiftVec 2 ?[t₁, t₂] = ?[L.termBShift t₁, L.termBShift t₂] := by
   rw [show (2 : V) = 0 + 1 + 1  by simp [one_add_one_eq_two], termBShiftVec_cons] <;> simp [*]
 
-@[simp] lemma Language.IsSemiterm.termBShift {t} (ht : L.IsSemiterm n t) : L.IsSemiterm (n + 1) (L.termBShift n t) := by
+@[simp] lemma Language.IsSemiterm.termBShift {t} (ht : L.IsSemiterm n t) : L.IsSemiterm (n + 1) (L.termBShift t) := by
   apply Language.IsSemiterm.induction 𝚺 ?_ ?_ ?_ ?_ t ht
   · definability
   · intro z hz; simp [hz]
   · intro x; simp
   · intro k f v hkf hv ih;
-    simp only [hkf, hv, termBShift_func, Language.IsSemiterm.func_iff, true_and]
-    exact ⟨by simp [Language.termBShiftVec, hv], fun i hi ↦ by
-      rw [nth_termBShiftVec hv hi]
-      exact ih i hi⟩
+    simp only [hkf, hv.isUTerm, termBShift_func, func, true_and]
+    refine Language.IsSemitermVec.iff.mpr ⟨?_, ?_⟩
+    · simp [hv.isUTerm]
+    · intro i hi
+      rw [nth_termBShiftVec hv.isUTerm hi]
+      exact ih i hi
 
-@[simp] lemma Language.IsSemitermVec.termBShiftVec {k n v} (hv : L.IsSemitermVec k n v) : L.IsSemitermVec k (n + 1) (L.termBShiftVec k n v) :=
-  ⟨by simp [Language.termBShiftVec, hv], fun i hi ↦ by
-    rw [nth_termBShiftVec hv hi]
-    exact (hv.prop hi).termBShift⟩
+@[simp] lemma Language.IsSemitermVec.termBShiftVec {k n v} (hv : L.IsSemitermVec k n v) : L.IsSemitermVec k (n + 1) (L.termBShiftVec k v) :=
+  Language.IsSemitermVec.iff.mpr
+  ⟨by simp [hv.isUTerm], fun i hi ↦ by
+    rw [nth_termBShiftVec hv.isUTerm hi]; exact (hv.nth hi).termBShift⟩
 
-lemma termBShift_termShift {t} (ht : L.IsSemiterm n t) : L.termBShift n (L.termShift n t) = L.termShift (n + 1) (L.termBShift n t) := by
+lemma termBShift_termShift {t} (ht : L.IsSemiterm n t) : L.termBShift (L.termShift t) = L.termShift (L.termBShift t) := by
   apply Language.IsSemiterm.induction 𝚺 ?_ ?_ ?_ ?_ t ht
   · definability
   · intro z hz; simp [hz]
   · intro x; simp
   · intro k f v hkf hv ih
-    simp only [termShift_func, Language.IsSemitermVec.termShiftVec, termBShift_func,
-      Language.IsSemitermVec.termBShiftVec, qqFunc_inj, true_and, hkf, hv]
-    apply nth_ext' k (by simp [hv]) (by simp [hv])
+    rw [L.termShift_func hkf hv.isUTerm,
+      L.termBShift_func hkf hv.termShiftVec.isUTerm,
+      L.termBShift_func hkf hv.isUTerm,
+      L.termShift_func hkf hv.termBShiftVec.isUTerm]
+    simp only [qqFunc_inj, true_and]
+    apply nth_ext' k
+      (by rw [len_termBShiftVec hv.termShiftVec.isUTerm]) (by rw [len_termShiftVec hv.termBShiftVec.isUTerm])
     intro i hi
-    rw [nth_termBShiftVec hv.termShiftVec hi, nth_termShiftVec hv hi,
-      nth_termShiftVec hv.termBShiftVec hi, nth_termBShiftVec hv hi, ih i hi]
+    rw [nth_termBShiftVec hv.termShiftVec.isUTerm hi, nth_termShiftVec hv.isUTerm hi,
+      nth_termShiftVec hv.termBShiftVec.isUTerm hi, nth_termBShiftVec hv.isUTerm hi, ih i hi]
 
 end termBShift
 
 variable (L)
 
-def Language.qVec (k n w : V) : V := ^#0 ∷ L.termBShiftVec k n w
+def Language.qVec (k w : V) : V := ^#0 ∷ L.termBShiftVec k w
 
 variable {L}
 
-@[simp] lemma len_qVec {k n w : V} (h : L.IsSemitermVec k n w) : len (L.qVec k n w) = k + 1 := by simp [Language.qVec, h]
+@[simp] lemma len_qVec {k w : V} (h : L.IsUTermVec k w) : len (L.qVec k w) = k + 1 := by simp [Language.qVec, h]
 
-lemma Language.IsSemitermVec.qVec {k n w : V} (h : L.IsSemitermVec k n w) : L.IsSemitermVec (k + 1) (n + 1) (L.qVec k n w) :=
-  ⟨by simp [h], by
-      intro i hi
-      rcases zero_or_succ i with (rfl | ⟨i, rfl⟩)
-      · simp [Language.qVec]
-      · simpa [Language.qVec, nth_termBShiftVec h (by simpa using hi)] using
-          h.prop (by simpa using hi) |>.termBShift⟩
+lemma Language.IsSemitermVec.qVec {k n w : V} (h : L.IsSemitermVec k n w) : L.IsSemitermVec (k + 1) (n + 1) (L.qVec k w) := by
+  refine Language.IsSemitermVec.iff.mpr ⟨?_, ?_⟩
+  · simp [h.isUTerm]
+  · intro i hi
+    rcases zero_or_succ i with (rfl | ⟨i, rfl⟩)
+    · simp [Language.qVec]
+    · simpa [Language.qVec, nth_termBShiftVec h.isUTerm (by simpa using hi)] using
+        h.nth (by simpa using hi) |>.termBShift
 
-lemma substs_cons_bShift {n m u t w} (ht : L.IsSemiterm n t) (hw : L.IsSemitermVec n m w) :
-    L.termSubst (n + 1) m (u ∷ w) (L.termBShift n t) = L.termSubst n m w t := by
+lemma substs_cons_bShift {u t w} (ht : L.IsSemiterm n t) :
+    L.termSubst (u ∷ w) (L.termBShift t) = L.termSubst w t := by
   apply Language.IsSemiterm.induction 𝚺 ?_ ?_ ?_ ?_ t ht
   · definability
   · intro z hz; simp [hz]
   · intro x; simp
   · intro k f v hf hv ih
-    simp [hf, hv]
-    apply nth_ext' k (by simp [hv, hw]) (by simp [hv, hw])
+    rw [Language.termBShift_func hf hv.isUTerm,
+      Language.termSubst_func hf hv.termBShiftVec.isUTerm,
+      Language.termSubst_func hf hv.isUTerm]
+    simp [hf, hv.isUTerm]
+    apply nth_ext' k
+      (by rw [len_termSubstVec hv.termBShiftVec.isUTerm])
+      (by rw [len_termSubstVec hv.isUTerm])
     intro i hi
-    simp [nth_termSubstVec hv.termBShiftVec hi, nth_termSubstVec hv hi, nth_termBShiftVec hv hi, ih i hi]
+    rw [nth_termSubstVec hv.termBShiftVec.isUTerm hi,
+      nth_termSubstVec hv.isUTerm hi,
+      nth_termBShiftVec hv.isUTerm hi,
+      ih i hi]
 
 lemma termShift_termSubsts {n m w t} (ht : L.IsSemiterm n t) (hw : L.IsSemitermVec n m w) :
-    L.termShift m (L.termSubst n m w t) = L.termSubst n m (L.termShiftVec n m w) (L.termShift n t) := by
+    L.termShift (L.termSubst w t) = L.termSubst (L.termShiftVec n w) (L.termShift t) := by
   apply Language.IsSemiterm.induction 𝚺 ?_ ?_ ?_ ?_ t ht
   · definability
-  · intro z hz; simp [hz, nth_termShiftVec hw hz]
+  · intro z hz; simp [nth_termShiftVec hw.isUTerm hz]
   · intro x; simp
   · intro k f v hf hv ih
-    simp only [termSubst_func, Language.IsSemitermVec.termSubstVec, termShift_func,
-      Language.IsSemitermVec.termShiftVec, qqFunc_inj, true_and, hf, hv, hw]
-    apply nth_ext' k (by simp [hw, hv]) (by simp [hv])
+    rw [L.termSubst_func hf hv.isUTerm,
+      L.termShift_func hf (hw.termSubstVec hv).isUTerm,
+      L.termShift_func hf hv.isUTerm,
+      L.termSubst_func hf hv.termShiftVec.isUTerm]
+    simp only [qqFunc_inj, true_and]
+    apply nth_ext' k
+      (by rw [len_termShiftVec (hw.termSubstVec hv).isUTerm])
+      (by rw [len_termSubstVec hv.termShiftVec.isUTerm])
     intro i hi
-    rw [nth_termShiftVec (hw.termSubstVec hv) hi,
-      nth_termSubstVec hv hi,
-      nth_termSubstVec hv.termShiftVec hi,
-      nth_termShiftVec hv hi, ih i hi]
+    rw [nth_termShiftVec (hw.termSubstVec hv).isUTerm hi,
+      nth_termSubstVec hv.isUTerm hi,
+      nth_termSubstVec hv.termShiftVec.isUTerm hi,
+      nth_termShiftVec hv.isUTerm hi, ih i hi]
 
 lemma bShift_substs {n m w t} (ht : L.IsSemiterm n t) (hw : L.IsSemitermVec n m w) :
-    L.termBShift m (L.termSubst n m w t) = L.termSubst n (m + 1) (L.termBShiftVec n m w) t := by
+    L.termBShift (L.termSubst w t) = L.termSubst (L.termBShiftVec n w) t := by
   apply Language.IsSemiterm.induction 𝚺 ?_ ?_ ?_ ?_ t ht
   · definability
-  · intro z hz; simp [hz, nth_termBShiftVec hw hz]
+  · intro z hz; simp [hz, nth_termBShiftVec hw.isUTerm hz]
   · intro x; simp
   · intro k f v hf hv ih
-    simp only [hf, hv, termSubst_func, hw.termSubstVec hv, termBShift_func, qqFunc_inj, true_and]
-    apply nth_ext' k (by simp [hw, hv]) (by simp [hv])
+    rw [L.termSubst_func hf hv.isUTerm,
+      L.termBShift_func hf (hw.termSubstVec hv).isUTerm,
+      L.termSubst_func hf hv.isUTerm]
+    simp only [qqFunc_inj, true_and]
+    apply nth_ext' k
+      (by rw [len_termBShiftVec (hw.termSubstVec hv).isUTerm])
+      (by rw [len_termSubstVec hv.isUTerm])
     intro i hi
-    simp [nth_termBShiftVec (hw.termSubstVec hv) hi, nth_termSubstVec hv hi, ih i hi]
+    simp [nth_termBShiftVec (hw.termSubstVec hv).isUTerm hi, nth_termSubstVec hv.isUTerm hi, ih i hi]
 
 lemma substs_qVec_bShift {n t m w} (ht : L.IsSemiterm n t) (hw : L.IsSemitermVec n m w) :
-    L.termSubst (n + 1) (m + 1) (L.qVec n m w) (L.termBShift n t) = L.termBShift m (L.termSubst n m w t) := by
-  simp [Language.qVec, substs_cons_bShift ht hw.termBShiftVec, bShift_substs ht hw]
+    L.termSubst (L.qVec n w) (L.termBShift t) = L.termBShift (L.termSubst w t) := by
+  simp [Language.qVec]
+  rw [substs_cons_bShift ht, bShift_substs ht hw]
 
 lemma termSubstVec_qVec_qVec {l n m : V} (hv : L.IsSemitermVec l n v) (hw : L.IsSemitermVec n m w) :
-    L.termSubstVec (l + 1) (n + 1) (m + 1) (L.qVec n m w) (L.qVec l n v) = L.qVec l m (L.termSubstVec l n m w v) := by
-  apply nth_ext' (l + 1) (by rw[len_termSubstVec hv.qVec]) (by simp [hw, hv])
+    L.termSubstVec (l + 1) (L.qVec n w) (L.qVec l v) = L.qVec l (L.termSubstVec l w v) := by
+  apply nth_ext' (l + 1)
+    (by rw [len_termSubstVec hv.qVec.isUTerm])
+    (by rw [len_qVec (hw.termSubstVec hv).isUTerm])
   intro i hi
   unfold Language.qVec
-  rw [termSubstVec_cons (by simp) hv.termBShiftVec]
+  rw [termSubstVec_cons (by simp) hv.termBShiftVec.isUTerm]
   rcases zero_or_succ i with (rfl | ⟨i, rfl⟩)
   · simp
   · simp
     have hi : i < l := by simpa using hi
-    rw [nth_termSubstVec hv.termBShiftVec hi,
-      nth_termBShiftVec hv hi,
-      nth_termBShiftVec (hw.termSubstVec hv) hi,
-      nth_termSubstVec hv hi,
-      substs_cons_bShift (hv.2 i hi) hw.termBShiftVec,
-      bShift_substs (hv.2 i hi) hw]
+    rw [nth_termSubstVec hv.termBShiftVec.isUTerm hi,
+      nth_termBShiftVec hv.isUTerm hi,
+      nth_termBShiftVec (hw.termSubstVec hv).isUTerm hi,
+      nth_termSubstVec hv.isUTerm hi,
+      substs_cons_bShift (hv.nth hi),
+      bShift_substs (hv.nth hi) hw]
 
 lemma termShift_qVec {n m w : V} (hw : L.IsSemitermVec n m w) :
-    L.termShiftVec (n + 1) (m + 1) (L.qVec n m w) = L.qVec n m (L.termShiftVec n m w) := by
-  apply nth_ext' (n + 1) (by rw [len_termShiftVec hw.qVec]) (by simp [hw])
+    L.termShiftVec (n + 1) (L.qVec n w) = L.qVec n (L.termShiftVec n w) := by
+  apply nth_ext' (n + 1)
+    (by rw [len_termShiftVec hw.qVec.isUTerm])
+    (by rw [len_qVec hw.termShiftVec.isUTerm])
   intro i hi
-  rw [nth_termShiftVec hw.qVec hi]
+  rw [nth_termShiftVec hw.qVec.isUTerm hi]
   unfold Language.qVec
   rcases zero_or_succ i with (rfl | ⟨i, rfl⟩)
   · simp
   · rw [nth_cons_succ, nth_cons_succ,
-      nth_termBShiftVec hw (by simpa using hi),
-      nth_termBShiftVec hw.termShiftVec (by simpa using hi),
-      nth_termShiftVec hw (by simpa using hi),
-      termBShift_termShift (hw.2 i (by simpa using hi))]
+      nth_termBShiftVec hw.isUTerm (by simpa using hi),
+      nth_termBShiftVec hw.termShiftVec.isUTerm (by simpa using hi),
+      nth_termShiftVec hw.isUTerm (by simpa using hi),
+      termBShift_termShift (hw.nth (by simpa using hi))]
 
 section fvfree
 
 variable (L)
 
-def Language.IsTermFVFree (n t : V) : Prop := L.IsSemiterm n t ∧ L.termShift n t = t
+def Language.IsTermFVFree (n t : V) : Prop := L.IsSemiterm n t ∧ L.termShift t = t
 
 variable {L}
 
 @[simp] lemma Language.IsTermFVFree.bvar (x : V) : L.IsTermFVFree n ^#x ↔ x < n := by
   simp [Language.IsTermFVFree]
-  intro h; simp [h]
 
 @[simp] lemma Language.IsTermFVFree.fvar (x : V) : ¬L.IsTermFVFree n ^&x := by
   simp [Language.IsTermFVFree]
@@ -536,9 +557,9 @@ lemma qqAdd_defined : 𝚺₁-Function₂ (qqAdd : V → V → V) via qqAddDef :
 lemma qqMul_defined : 𝚺₁-Function₂ (qqMul : V → V → V) via qqMulDef := by
   intro v; simp [qqMulDef, numeral_eq_natCast, qqMul]
 
-instance (Γ m) : Γ-[m + 1]-Function₂ (qqAdd : V → V → V) := .of_sigmaOne qqAdd_defined.to_definable _ _
+instance : Γ-[m + 1]-Function₂ (qqAdd : V → V → V) := .of_sigmaOne qqAdd_defined.to_definable
 
-instance (Γ m) : Γ-[m + 1]-Function₂ (qqMul : V → V → V) := .of_sigmaOne qqMul_defined.to_definable _ _
+instance : Γ-[m + 1]-Function₂ (qqMul : V → V → V) := .of_sigmaOne qqMul_defined.to_definable
 
 end
 
@@ -553,10 +574,8 @@ lemma qqFunc_absolute (k f v : ℕ) : ((^func k f v : ℕ) : V) = ^func (k : V) 
 namespace Numeral
 
 def blueprint : PR.Blueprint 0 where
-  zero := .mkSigma “y | y = !!(IsSemiterm.Operator.numeral ℒₒᵣ Formalized.one)” (by simp)
-  succ := .mkSigma “y t n | ∃ p,
-    !mkVec₂Def p t !!(IsSemiterm.Operator.numeral ℒₒᵣ Formalized.one) ∧
-    !qqFuncDef y 2 !!(IsSemiterm.Operator.numeral ℒₒᵣ addIndex) p” (by simp)
+  zero := .mkSigma “y | y = ↑Formalized.one” (by simp)
+  succ := .mkSigma “y t n | ∃ p, !mkVec₂Def p t ↑Formalized.one ∧ !qqFuncDef y 2 ↑addIndex p” (by simp)
 
 def construction : PR.Construction V blueprint where
   zero := fun _ ↦ 𝟏
@@ -612,11 +631,13 @@ lemma numeral_succ_pos (pos : 0 < n) : numeral (n + 1 : V) = numeral n ^+ 𝟏 :
 @[simp] lemma numeral_semiterm (n x : V) : ⌜ℒₒᵣ⌝.IsSemiterm n (numeral x) := by
   by_cases hx : x = 0 <;> simp [hx, numeral]
 
+@[simp] lemma numeral_uterm (x : V) : ⌜ℒₒᵣ⌝.IsUTerm (numeral x) := (numeral_semiterm 0 x).isUTerm
+
 section
 
 def _root_.LO.FirstOrder.Arith.numeralDef : 𝚺₁.Semisentence 2 := .mkSigma
   “t x |
-    (x = 0 → t = !!(IsSemiterm.Operator.numeral ℒₒᵣ Formalized.zero)) ∧
+    (x = 0 → t = ↑Formalized.zero) ∧
     (x ≠ 0 → ∃ x', !subDef x' x 1 ∧ !numeralAuxDef t x')”
   (by simp)
 
@@ -627,34 +648,38 @@ lemma numeral_defined : 𝚺₁-Function₁ (numeral : V → V) via numeralDef :
 @[simp] lemma eval_numeralDef (v) :
     Semiformula.Evalbm V v numeralDef.val ↔ v 0 = numeral (v 1) := numeral_defined.df.iff v
 
-@[simp] instance numeral_definable : 𝚺₁-Function₁ (numeral : V → V) := numeral_defined.to_definable
+instance numeral_definable : 𝚺₁-Function₁ (numeral : V → V) := numeral_defined.to_definable
 
-@[simp] instance numeral_definable' (Γ m) : Γ-[m + 1]-Function₁ (numeral : V → V) := .of_sigmaOne numeral_definable _ _
+instance numeral_definable' : Γ-[m + 1]-Function₁ (numeral : V → V) := .of_sigmaOne numeral_definable
 
 end
 
 @[simp] lemma numeral_substs {w : V} (hw : ⌜ℒₒᵣ⌝.IsSemitermVec n m w) (x : V) :
-    ⌜ℒₒᵣ⌝.termSubst n m w (numeral x) = numeral x := by
+    ⌜ℒₒᵣ⌝.termSubst w (numeral x) = numeral x := by
   induction x using induction_sigma1
   · definability
   case zero => simp [hw, Formalized.zero, qqFunc_absolute]
   case succ x ih =>
     rcases zero_or_succ x with (rfl | ⟨x, rfl⟩)
     · simp [hw, Formalized.one, qqFunc_absolute]
-    · simp [qqAdd, hw, ih, Formalized.one, qqFunc_absolute]
+    · simp only [numeral_add_two, qqAdd, LOR_func_addIndex]
+      rw [Language.termSubst_func (by simp) (by simp [Formalized.one, qqFunc_absolute])]
+      simp [ih, Formalized.one, qqFunc_absolute]
 
 @[simp] lemma numeral_shift (x : V) :
-    ⌜ℒₒᵣ⌝.termShift n (numeral x) = numeral x := by
+    ⌜ℒₒᵣ⌝.termShift (numeral x) = numeral x := by
   induction x using induction_sigma1
   · definability
   case zero => simp [Formalized.zero, qqFunc_absolute]
   case succ x ih =>
     rcases zero_or_succ x with (rfl | ⟨x, rfl⟩)
     · simp [Formalized.one, qqFunc_absolute]
-    · simp [qqAdd, ih, Formalized.one, qqFunc_absolute]
+    · simp only [numeral_add_two, qqAdd, LOR_func_addIndex]
+      rw [Language.termShift_func (by simp) (by simp [Formalized.one, qqFunc_absolute])]
+      simp [ih, Formalized.one, qqFunc_absolute]
 
 @[simp] lemma numeral_bShift (x : V) :
-    ⌜ℒₒᵣ⌝.termBShift n (numeral x) = numeral x := by
+    ⌜ℒₒᵣ⌝.termBShift (numeral x) = numeral x := by
   induction x using induction_sigma1
   · definability
   case zero => simp [Formalized.zero, qqFunc_absolute]
